progress towards auth code secrecy

examples/webmodel/OAuth.Formal.fst
@@ -19,8 +19,9 @@ assume val includes: i:index -> o:origin -> GTot Type
 
 assume val index2 : o1:origin -> o2:origin -> i:index{includes i o1 /\ includes i o2}
 
-type nonce (idx:index)
-assume val eq_nonce: #(idx:index) -> nonce idx -> nonce idx -> bool
+type nonce
+assume val nonce_index: nonce -> index
+assume val eq_nonce: x:nonce -> y:nonce -> b:bool{b ==> nonce_index x == nonce_index y}
 
 assume val param_index: param -> GTot index
 type pub_param = p:param{param_index p == public_index}
@@ -31,7 +32,7 @@ type pub_header = h:header{header_index h == public_index}
 assume val body_index: body -> GTot index
 type pub_body = b:body{body_index b == public_index}
 
-assume val can_send_public: i:index -> Lemma 
+assume val can_send_public: i:index ->  Lemma 
 	   (requires True)
 	   (ensures (fun _ -> can_send public_index i))
 	   [SMTPat (can_send public_index i)]
@@ -44,13 +45,13 @@ assume val request_path: http_request -> string
 assume val request_method: http_request -> string
 assume val request_parameters: http_request -> (list param)
 assume val request_origin_header: http_request -> string
-assume val request_cookie_header: #idx:index -> http_request -> nonce idx
+assume val request_cookie_header: http_request -> nonce
 assume val request_body: http_request -> body
 
 
 assume val mk_referrer_policy_header: string -> header
-assume val mk_set_cookie_header: #idx:index -> nonce idx -> header
-assume val mk_authorization_header: #idx:index -> string -> nonce idx -> header
+assume val mk_set_cookie_header: n:nonce -> h:header{header_index h == nonce_index n}
+assume val mk_authorization_header: string -> n:nonce -> h:header{header_index h == nonce_index n}
 
 assume val mk_request: #req_idx:index -> 
 		       method:string -> 
@@ -79,19 +80,26 @@ unfold let return (x:'a) : server 'a =
   fun s0 -> x,s0
 
 type session
-assume val create_session: #idx:index -> server (nonce idx)
-assume val mk_nonce: #idx:index -> server (nonce idx)
+assume val create_session: server nonce
+assume val mk_nonce: server nonce
 
 // OAuth Specific
 type idp_record
-assume val read_idps: origin -> server (list idp_record) 
 assume val get_idp_origin: idp_record -> origin
-assume val get_idp_record: o:origin -> list idp_record -> option (ir:idp_record{get_idp_origin ir == o})
+assume val get_rp_origin: idp_record -> origin
+//assume val read_idps: o:origin -> server (list (ir:idp_record{get_rp_origin ir == o})) 
+//assume val get_idp_record: o:origin -> list idp_record -> option (ir:idp_record{get_idp_origin ir == o})
+assume val read_idp_record: rp:origin -> ip:origin -> server (option (ir:idp_record{get_rp_origin ir == rp /\ get_idp_origin ir == ip}))
+
 assume val get_idp_auth_endpoint_uri: ir:idp_record -> u:uri{uri_origin u == get_idp_origin ir}
 assume val get_idp_token_endpoint_uri: ir:idp_record -> u:uri{uri_origin u == get_idp_origin ir}
 assume val get_idp_introspection_endpoint_uri: ir:idp_record -> u:uri{uri_origin u == get_idp_origin ir}
 assume val get_client_id: idp_record -> string
-assume val get_client_secret: #idx:index -> idp_record -> option (nonce idx)
+assume val get_client_secret: ir:idp_record -> option (n:nonce{nonce_index n `includes` get_rp_origin ir /\ 
+							      nonce_index n `includes` get_idp_origin ir /\
+							      can_send (nonce_index n) 
+								(index2 (get_idp_origin ir) (get_rp_origin ir))})
+
 
 assume val response_type_param: string -> pub_param
 assume val client_id_param: string -> pub_param
@@ -99,32 +107,46 @@ assume val idp_param: origin -> pub_param
 assume val redirect_uri_param: uri -> pub_param
 assume val script_param: string -> pub_param
 assume val grant_type_param: string -> pub_param
+assume val state_param: n:nonce -> p:param{param_index p == nonce_index n}
+assume val authorization_code_param: n:nonce -> p:param{param_index p == nonce_index n}
+assume val access_token_param: n:nonce -> p:param{param_index p == nonce_index n}
 
-assume val state_param: #idx:index -> nonce idx -> p:param{param_index p == idx}
-assume val authorization_code_param: #idx:index -> nonce idx -> p:param{param_index p == idx}
-assume val access_token_param: #idx:index -> nonce idx -> p:param{param_index p == idx}
+// Any IP/RP/User is only allowed to create a "code" parameter in a URI or message body using this function
+assume val idp_code_params: user:uid -> ip:origin -> rp:origin -> code:nonce -> Pure param
+			    (requires (nonce_index code == public_index \/
+				       (nonce_index code `includes` ip /\
+					nonce_index code `includes` rp /\
+				        nonce_index code `includes` user /\
+				        can_send (nonce_index code) (index2 ip rp))))
+			    (ensures (fun _ -> True))
 
 assume val get_idp_param: (list param) -> option origin
 assume val get_client_id_param: (list param) -> option string
-assume val get_state_param: #idx:index -> (list param) -> option (nonce idx)
+assume val get_state_param: (list param) -> option nonce 
 assume val get_mode_param: (list param) -> option string // echoes back response_type
-assume val get_code_param: #idx:index -> (list param) -> option (nonce idx)
-assume val get_access_token_param: #idx:index -> (list param) -> option (nonce idx)
+assume val get_code_param: (list param) -> option nonce 
+assume val get_access_token_param: (list param) -> option nonce
 
-(*
-assume val get_idp_code_params: #idx:index -> (list param) -> Pure (option (origin * nonce idx))
-					   (requires True)
-					   (ensures (fun x -> match x with 
-							   | None -> True
-							   | Some (idp,code) -> 
-*)
-assume val set_rp_session: #idx:index -> #idx':index -> loginSessionId:nonce idx -> idp:origin -> s:nonce idx' -> m:string -> redir:uri -> server unit
-assume val get_rp_session: #idx:index -> #idx':index -> loginSessionId:nonce idx -> server (option (idp:origin * s:nonce idx' * m:string * redir:uri))
+// Postcondition can be proved using an invariant on the "code" parameter, relying on the precondition on idp_code_params
+assume val get_idp_code_params: (rp:origin) -> (list param) -> Pure (option (origin * nonce))
+				   (requires True)
+				   (ensures (fun x -> match x with 
+						   | None -> True
+						   | Some (idp,code) -> 
+						     nonce_index code == public_index \/
+						     (nonce_index code `includes` idp /\
+						      nonce_index code `includes` rp /\
+						      can_send (nonce_index code) (index2 idp rp))))
 
-assume val set_rp_request_state: #idx:index -> #idx':index -> request_id:nonce idx -> mode:string -> idp:origin -> req:nonce idx' -> server unit
-assume val get_rp_request_state: #idx:index -> #idx':index -> request_id:nonce idx -> server (option (mode:string * idp:origin * req:nonce idx'))
+assume val set_rp_session: loginSessionId:nonce -> idp:origin -> s:nonce -> m:string -> redir:uri -> server unit
+assume val get_rp_session: loginSessionId:nonce -> server (option (idp:origin * s:nonce * m:string * redir:uri))
 
-noeq type http_message = | Req : #idx:index -> id:nonce idx -> http_request -> http_message | Resp: #idx:index -> id:nonce idx -> http_response -> http_message
+assume val set_rp_request_state: request_id:nonce -> mode:string -> idp:origin -> req:nonce -> server unit
+assume val get_rp_request_state: request_id:nonce -> server (option (mode:string * idp:origin * req:nonce))
+
+noeq type http_message = 
+  | Req : id:nonce -> http_request -> http_message 
+  | Resp: id:nonce -> http_response -> http_message
 
 #reset-options "--z3rlimit 100"
 //val rp_http_server: rp_origin:origin -> msg:http_message -> server (option (msg':http_message{
@@ -135,14 +157,14 @@ noeq type http_message = | Req : #idx:index -> id:nonce idx -> http_request -> h
 
 let rp_http_server (rp_origin:origin) (msg:http_message) : server (option http_message) = 
  match msg with
- | Req #idx id req -> 
+ | Req id req -> 
   let path = request_path req in
   if path = "/" then
     let headers = [mk_referrer_policy_header "origin"] in 
     let script_ = script_param "script_rp_index" in
-    can_send_public idx;
-    assert (can_send (param_index script_) idx);
-    let resp = Resp #idx id (mk_response headers (mk_body #idx [script_])) in
+    can_send_public (nonce_index id);
+    assert (can_send (param_index script_) (nonce_index id));
+    let resp = Resp id (mk_response headers (mk_body #(nonce_index id) [script_])) in
     return (Some resp)
   else if path = "/startInteractiveLogin" then
     if (request_method req = "POST" &&
@@ -152,11 +174,11 @@ let rp_http_server (rp_origin:origin) (msg:http_message) : server (option http_m
        match get_idp_param (get_body (request_body req)) with
        | None -> return None 
        | Some idp -> 
-	 idps <-- read_idps rp_origin ;
-	 match get_idp_record idp idps with
+	 iro <-- read_idp_record rp_origin idp;
+	 match iro with
 	 | None -> return None
 	 | Some ir -> 
-	   (state <-- mk_nonce #idx ;
+	   (state <-- mk_nonce ;
 	     let auth_uri = get_idp_auth_endpoint_uri ir in
 	     let client_id = get_client_id ir in
 	     let redirect_uri = mk_uri rp_origin "/redirectionEndpoint" [idp_param idp] in
@@ -164,64 +186,74 @@ let rp_http_server (rp_origin:origin) (msg:http_message) : server (option http_m
 						    client_id_param client_id; 
 						    state_param state; 
 						    redirect_uri_param redirect_uri] in
-	     session_id <-- create_session #idx ;
+	     session_id <-- create_session ;
 	     set_rp_session session_id idp state "code" redirect_uri ;;
 	     let resp = mk_redirect_response auth_uri [mk_set_cookie_header session_id; mk_referrer_policy_header "origin"] in
-	     let resp = Resp #idx id resp in 
+	     let resp = Resp id resp in 
 	     return (Some resp)))
 	     else return None
     else if path = "/redirectionEndpoint" then
       let session_id = request_cookie_header req in
-      session_or_none <-- get_rp_session #idx #idx session_id ;
+      session_or_none <-- get_rp_session session_id ;
       match session_or_none with
       | None -> return None
       | Some (idp, state, mode, redir) -> 
-	idps <-- read_idps rp_origin ;
-	match get_idp_record idp idps with
+	iro <-- read_idp_record rp_origin idp;
+	match iro with
 	| None -> return None
 	| Some ir -> 
 	       let client_id = get_client_id ir in
 	       let req_params = request_parameters req in
-	       match (get_client_id_param req_params, 
-		     get_idp_param req_params, 
-		     get_state_param #idx req_params,
-		     get_mode_param req_params) with
-               | Some cid, Some idp', Some state', Some mode ->
-		      if (cid = client_id && idp' = idp && eq_nonce state state' && mode = "code") then  
+	       
+	       match (get_client_id_param req_params, get_state_param req_params, get_mode_param req_params) with
+               | Some cid, Some st, Some mode ->
+	           if (cid = client_id && eq_nonce st state && mode = "code") then  
 			      // be careful of side-channel leaks in state = state'
-	              match (get_code_param #idx req_params) with
+	              match (get_idp_code_params rp_origin req_params) with
 		      | None -> return None
-		      | Some code -> 
-                             match (get_client_secret #idx ir) with
+		      | Some (idp', code) -> 
+			  if (idp' <> idp) then 
+			    return None 
+			  else
+                             match (get_client_secret ir) with
 			     | None -> return None
 			     | Some sec -> 
 				    let token_index = index2 idp rp_origin in
+				    let auth_header = mk_authorization_header client_id sec in
+				    let grant_param = grant_type_param "authorization_code" in
+				    can_send_public token_index;
+				    assert(can_send (param_index grant_param) token_index);
+
+				    let code_param = authorization_code_param code in
+				    assert(can_send (param_index code_param) token_index);
+				    
 				    let token_request = mk_request #token_index "POST" 
+				    
 							(get_idp_token_endpoint_uri ir)
-							[mk_authorization_header client_id sec] 
+							[auth_header] 
 							(mk_body #token_index 
-								 [grant_type_param "authorization_code";
+								 [grant_param;
 							          authorization_code_param code;
 								  redirect_uri_param redir]) in
 				    request_id <-- mk_nonce ;
 				    set_rp_request_state request_id "code" idp id ;;
-			            return (Some (Req #idx request_id token_request))
+			            return (Some (Req request_id token_request))
     
 		      else return None   
-	       | _,_,_,_ -> return None
+	       | _,_,_ -> return None
     else return None
- | Resp #idx id resp -> // process IP's response and process API response
+ | Resp id resp -> // process IP's response and process API response
      session_or_none <-- get_rp_request_state id ;
      match session_or_none with
      | None -> return None
      | Some (mode,idp,prev) -> 
         if mode = "code" then 
         let resp_params = get_body (response_body resp) in
-	match get_access_token_param #idx resp_params with
+	match get_access_token_param resp_params with
 	| None -> return None
 	| Some token -> 
-	  idps <-- read_idps rp_origin ;
-	  match get_idp_record idp idps with
+	  iro <-- read_idp_record rp_origin idp;
+	  match iro with
 	  | None -> return None
 	  | Some ir -> 
 		 let intros_uri = get_idp_introspection_endpoint_uri ir in
@@ -232,15 +264,15 @@ let rp_http_server (rp_origin:origin) (msg:http_message) : server (option http_m
 		 assert (includes request_idx idp);
 		 assert (includes request_idx (uri_origin intros_uri));
 		 let request = mk_request #request_idx "GET" intros_uri [] (mk_body #request_idx []) in
-		 return (Some (Req #idx request_id request))
+		 return (Some (Req request_id request))
         else if mode = "introspect" then
 	     /// We may get back the userid and/or a protected resource and/or client_id here
 	     /// For authentication, we need to check these values, but not for authorization
 	     let headers = [mk_referrer_policy_header "origin"] in 
 	     let script_ = script_param "script_rp_index" in
-	     can_send_public idx;
-	     assert (can_send (param_index script_) idx);
-	     return (Some (Resp #idx prev (mk_response headers (mk_body #idx [script_]))))
+	     can_send_public (nonce_index id);
+	     assert (can_send (param_index script_) (nonce_index id));
+	     return (Some (Resp prev (mk_response headers (mk_body #(nonce_index id) [script_]))))
 	else return None 
 
 
